\documentclass{article}
\usepackage{amsmath}
\begin{document}
    \begin{center}
        p = sum of $XY$, d = sum of $X^2$, w = sum of $Y^2$
    \end{center}
    \begin{align*}
        r&=\frac{p-n(\overline{x})(\overline{y})}{\sqrt{(d-n(\overline{x})^2)(w-n(\overline{y})^2)}}\\
        r&=\frac{15282-5(35.2)(86)}{\sqrt{(7016-5(35.2)^2)(37020-5(86)^2)}}\\
        r&=\frac{146}{\sqrt{(820)(40)}}\\
        r&=\frac{146}{181.1960264}\\
        r&= 0.805757183
    \end{align*}
    \begin{align*}
        t&=r\cdot \sqrt{\frac{n-2}{1-r^2}}\\
        t&=.81\cdot \sqrt{\frac{5-2}{1-.81^2}}\\
        t&=.81\cdot \sqrt{8.723466124}\\
        t&=.81\cdot 2.953551443\\
        t&=2.392376668
    \end{align*}
    \begin{center}
        d = sum of $D^2$
    \end{center}
    \begin{align*}
        \rho&=1-\frac{6(d)}{n(n^2-1)}\\
        \rho&=1-\frac{6(2)}{5(5^2-1)}\\
        \rho&=1-\frac{12}{120}\\ 
        \rho&=1-0.1\\
        \rho&=0.9
    \end{align*}
\end{document}
